Protocol/Variables.thy
@@ -2,11 +2,11 @@ theory Variables
   imports Main
 begin
 (* Variables - SLOTZERO *)
-type_synonym Transactions = int
-type_synonym Hash = int
-type_synonym Party = int
+type_synonym Transactions = nat
+type_synonym Hash = nat
+type_synonym Party = nat
 
-type_synonym Slot = int
+type_synonym Slot = nat
 definition "(SlotZero::int) = 0"
 
 type_synonym Delay = nat
